back to lax after PR 151

proofs/fstar/extraction-edited/Libcrux.Kem.Kyber.Hash_functions.fst
@@ -18,31 +18,96 @@ let v_PRF (v_LEN: usize) (input: t_Slice u8) =
   admit(); // We assume that sha3_512 correctly implements H
   res
 
-let v_XOFx4 (v_LEN v_K: usize) (input: t_Array (t_Array u8 (sz 34)) v_K) =
-  let out:t_Array (t_Array u8 v_LEN) v_K =
-    Rust_primitives.Hax.repeat (Rust_primitives.Hax.repeat 0uy v_LEN <: t_Array u8 v_LEN) v_K
+let v_XOFx4 (v_K: usize) (input: t_Array (t_Array u8 (sz 34)) v_K) =
+  let out:t_Array (t_Array u8 (sz 840)) v_K =
+    Rust_primitives.Hax.repeat (Rust_primitives.Hax.repeat 0uy (sz 840) <: t_Array u8 (sz 840)) v_K
   in
-  let out:t_Array (t_Array u8 v_LEN) v_K =
-    Core.Iter.Traits.Iterator.f_fold (Core.Iter.Traits.Collect.f_into_iter ({
-              Core.Ops.Range.f_start = sz 0;
-              Core.Ops.Range.f_end = v_K
-            }
-            <:
-            Core.Ops.Range.t_Range usize)
-        <:
-        Core.Ops.Range.t_Range usize)
-      out
-      (fun out i ->
-          let out:t_Array (t_Array u8 v_LEN) v_K = out in
-          let i:usize = i in
-          Rust_primitives.Hax.Monomorphized_update_at.update_at_usize out
-            i
-            (Libcrux.Digest.shake128 v_LEN
-                (Rust_primitives.unsize (input.[ i ] <: t_Array u8 (sz 34)) <: t_Slice u8)
+  let out:t_Array (t_Array u8 (sz 840)) v_K =
+    if ~.(Libcrux_platform.simd256_support <: bool) || ~.false
+    then
+      Core.Iter.Traits.Iterator.f_fold (Core.Iter.Traits.Collect.f_into_iter ({
+                Core.Ops.Range.f_start = sz 0;
+                Core.Ops.Range.f_end = v_K
+              }
               <:
-              t_Array u8 v_LEN)
+              Core.Ops.Range.t_Range usize)
           <:
-          t_Array (t_Array u8 v_LEN) v_K)
+          Core.Ops.Range.t_Range usize)
+        out
+        (fun out i ->
+            let out:t_Array (t_Array u8 (sz 840)) v_K = out in
+            let i:usize = i in
+            Rust_primitives.Hax.Monomorphized_update_at.update_at_usize out
+              i
+              (Libcrux.Digest.shake128 (sz 840)
+                  (Rust_primitives.unsize (input.[ i ] <: t_Array u8 (sz 34)) <: t_Slice u8)
+                <:
+                t_Array u8 (sz 840))
+            <:
+            t_Array (t_Array u8 (sz 840)) v_K)
+    else
+      let out:t_Array (t_Array u8 (sz 840)) v_K =
+        match cast (v_K <: usize) <: u8 with
+        | 2uy ->
+          let d0, d1, _, _:(t_Array u8 (sz 840) & t_Array u8 (sz 840) & t_Array u8 (sz 840) &
+            t_Array u8 (sz 840)) =
+            Libcrux.Digest.shake128x4 (sz 840)
+              (Rust_primitives.unsize (input.[ sz 0 ] <: t_Array u8 (sz 34)) <: t_Slice u8)
+              (Rust_primitives.unsize (input.[ sz 1 ] <: t_Array u8 (sz 34)) <: t_Slice u8)
+              (Rust_primitives.unsize (input.[ sz 0 ] <: t_Array u8 (sz 34)) <: t_Slice u8)
+              (Rust_primitives.unsize (input.[ sz 1 ] <: t_Array u8 (sz 34)) <: t_Slice u8)
+          in
+          let out:t_Array (t_Array u8 (sz 840)) v_K =
+            Rust_primitives.Hax.Monomorphized_update_at.update_at_usize out (sz 0) d0
+          in
+          let out:t_Array (t_Array u8 (sz 840)) v_K =
+            Rust_primitives.Hax.Monomorphized_update_at.update_at_usize out (sz 1) d1
+          in
+          out
+        | 3uy ->
+          let d0, d1, d2, _:(t_Array u8 (sz 840) & t_Array u8 (sz 840) & t_Array u8 (sz 840) &
+            t_Array u8 (sz 840)) =
+            Libcrux.Digest.shake128x4 (sz 840)
+              (Rust_primitives.unsize (input.[ sz 0 ] <: t_Array u8 (sz 34)) <: t_Slice u8)
+              (Rust_primitives.unsize (input.[ sz 1 ] <: t_Array u8 (sz 34)) <: t_Slice u8)
+              (Rust_primitives.unsize (input.[ sz 2 ] <: t_Array u8 (sz 34)) <: t_Slice u8)
+              (Rust_primitives.unsize (input.[ sz 0 ] <: t_Array u8 (sz 34)) <: t_Slice u8)
+          in
+          let out:t_Array (t_Array u8 (sz 840)) v_K =
+            Rust_primitives.Hax.Monomorphized_update_at.update_at_usize out (sz 0) d0
+          in
+          let out:t_Array (t_Array u8 (sz 840)) v_K =
+            Rust_primitives.Hax.Monomorphized_update_at.update_at_usize out (sz 1) d1
+          in
+          let out:t_Array (t_Array u8 (sz 840)) v_K =
+            Rust_primitives.Hax.Monomorphized_update_at.update_at_usize out (sz 2) d2
+          in
+          out
+        | 4uy ->
+          let d0, d1, d2, d3:(t_Array u8 (sz 840) & t_Array u8 (sz 840) & t_Array u8 (sz 840) &
+            t_Array u8 (sz 840)) =
+            Libcrux.Digest.shake128x4 (sz 840)
+              (Rust_primitives.unsize (input.[ sz 0 ] <: t_Array u8 (sz 34)) <: t_Slice u8)
+              (Rust_primitives.unsize (input.[ sz 1 ] <: t_Array u8 (sz 34)) <: t_Slice u8)
+              (Rust_primitives.unsize (input.[ sz 2 ] <: t_Array u8 (sz 34)) <: t_Slice u8)
+              (Rust_primitives.unsize (input.[ sz 3 ] <: t_Array u8 (sz 34)) <: t_Slice u8)
+          in
+          let out:t_Array (t_Array u8 (sz 840)) v_K =
+            Rust_primitives.Hax.Monomorphized_update_at.update_at_usize out (sz 0) d0
+          in
+          let out:t_Array (t_Array u8 (sz 840)) v_K =
+            Rust_primitives.Hax.Monomorphized_update_at.update_at_usize out (sz 1) d1
+          in
+          let out:t_Array (t_Array u8 (sz 840)) v_K =
+            Rust_primitives.Hax.Monomorphized_update_at.update_at_usize out (sz 2) d2
+          in
+          let out:t_Array (t_Array u8 (sz 840)) v_K =
+            Rust_primitives.Hax.Monomorphized_update_at.update_at_usize out (sz 3) d3
+          in
+          out
+        | _ -> out
+      in
+      out
   in
-  admit(); // We should prove that v_XOFx4 correctly implements Keccakx4
+  admit(); //P-F
   out
