proofs/fstar/extraction-edited/Libcrux.Kem.Kyber.Kyber768.fsti
@@ -22,15 +22,12 @@ val decapsulate_768_
 val encapsulate_768_
       (public_key: Libcrux.Kem.Kyber.Types.t_KyberPublicKey (sz 1184))
       (randomness: t_Array u8 (sz 32))
-    : Pure (Core.Result.t_Result
-           (Libcrux.Kem.Kyber.Types.t_KyberCiphertext (sz 1088) & t_Array u8 (sz 32))
-            Libcrux.Kem.Kyber.Types.t_Error)
+    : Pure (Libcrux.Kem.Kyber.Types.t_KyberCiphertext (sz 1088) & t_Array u8 (sz 32))
       (requires True)
-      (ensures (fun res -> True))
+      (ensures (fun (ct,ss)-> (ct.f_value,ss) == Spec.Kyber.kyber768_encapsulate public_key.f_value randomness))
 
 val generate_key_pair_768_ (randomness: t_Array u8 (sz 64))
-    : Pure (Core.Result.t_Result (Libcrux.Kem.Kyber.Types.t_KyberKeyPair (sz 2400) (sz 1184))
-            Libcrux.Kem.Kyber.Types.t_Error )
+    : Pure (Libcrux.Kem.Kyber.Types.t_KyberKeyPair (sz 2400) (sz 1184))
       (requires (True))
-      (ensures (fun res -> True))
+      (ensures (fun kp -> (kp.f_sk.f_value,kp.f_pk.f_value) == Spec.Kyber.kyber768_generate_keypair randomness))
 
